LeanLangur.lean
@@ -1,3 +1,10 @@
 -- This module serves as the root of the `LeanLangur` library.
 -- Import modules here that should be built as part of the library.
 import LeanLangur.Basic
+import LeanLangur.People
+import LeanLangur.QuickSort
+import LeanLangur.Exercises.LabelledTree
+import LeanLangur.Largest
+import LeanLangur.Draft.SelectionSort
+import LeanLangur.PyFor
+import LeanLangur.LangurLeaps
